Move code around

old/Example.v
@@ -1,10 +1,13 @@
-Require Export
+Require Import
+  Coq.ZArith.ZArith
+  Lib
   Ty
   Exp
   Sub
   Sem
-  Eval
-  Norm.
+  Norm
+  Lang
+  Eval.
 
 From Equations Require Import Equations.
 Set Equations With UIP.
@@ -15,25 +18,264 @@ Section Example.
 
 Import ListNotations.
 
+Open Scope Ty_scope.
+Open Scope Z_scope.
+
+Inductive Pact := PactLang.     (* this is just a type-level tag *)
+
+Derive NoConfusion NoConfusionHom for Pact.
+
+Inductive PactTy := TyInteger.
+
+Derive NoConfusion NoConfusionHom for PactTy.
+
+Definition Pact_HostTypes : HostTypes Pact := {|
+  HostTy := PactTy;
+  HostTySem := λ ty,
+    match ty with
+    | TyInteger => Z
+    end
+|}.
+
+(*
+Definition ℤ := TyHost (H:=Pact_HostTypes) TyInteger.
+Arguments ℤ /.
+(* Definition ℝ := TyHost TyDecimal. *)
+(* Definition 𝕋 := TyHost TyTime. *)
+(* Definition 𝕊 := TyHost TyString. *)
+Definition 𝔹 := TyBool (H:=Pact_HostTypes).
+
+Inductive PactExp : Ty (H:=Pact_HostTypes) → Type :=
+  | PInteger : Z → PactExp ℤ
+  | FAdd     : PactExp (ℤ × ℤ ⟶ ℤ).
+
+Derive Signature NoConfusion Subterm for PactExp.
+
+Definition Pact_HostExprs : HostExprs Pact := {|
+  has_host_types := Pact_HostTypes;
+  HostExp := PactExp
+|}.
+
+Equations Pact_HostExpSem `(e : PactExp τ) : SemTy (H:=Pact_HostTypes) τ :=
+  Pact_HostExpSem (PInteger z) := z;
+  Pact_HostExpSem FAdd         := uncurry Z.add.
+
+Definition fun1 {Γ} `(f : SemTy dom → SemTy cod) (e : PactExp (dom ⟶ cod))
+           (v : Exp (H:=Pact_HostExprs) Γ dom) (V : ValueP v) : Exp Γ cod.
+Proof.
+  dependent destruction e.
+  - inv V.
+    inv X;  inv x0; rename H into x.
+    inv X0; inv x0; rename H into y.
+    exact (HostedVal (H:=Pact_HostExprs) (PInteger (f (x, y)))).
+Defined.
+
+Fail Equations PactF {Γ : Env (H:=Pact_HostExprs)}
+          {dom cod : Ty (H:=Pact_HostTypes)}
+          (e : PactExp (dom ⟶ cod)) :
+  ∀ v : Exp (H:=Pact_HostExprs) Γ dom,
+    ValueP (H:=Pact_HostExprs) v → Exp Γ cod :=
+  PactF FAdd := fun1 Z.add.
+
+Definition PactF {Γ : Env (H:=Pact_HostExprs)}
+           {dom cod : Ty (H:=Pact_HostTypes)}
+           (e : PactExp (dom ⟶ cod)) :
+  ∀ v : Exp (H:=Pact_HostExprs) Γ dom,
+    ValueP (H:=Pact_HostExprs) v → Exp Γ cod.
+Proof.
+  inversion e; subst.
+  - now apply fun1; auto; apply (uncurry Z.add).
+Defined.
+
+Instance Pact_HostExprsSem : HostExprsSem Pact := {|
+  has_host_exprs := Pact_HostExprs;
+  HostExpSem := @Pact_HostExpSem;
+  CallHost := @PactF;
+  Reduce := λ _ _ x,
+    match x with
+    | PInteger x => existT _ (HostedVal (H:=Pact_HostExprs) (PInteger x)) (HostedValP _)
+    | FAdd       => existT _ (HostedFun (H:=Pact_HostExprs) FAdd) (HostedFunP _)
+    end
+|}.
+
+Program Instance Pact_HostLang : HostLang Pact := {|
+  has_host_exprs_sem := Pact_HostExprsSem;
+|}.
+Next Obligation.
+  dependent destruction f.
+  (* FAdd *)
+  - dependent elimination H; reduce.
+    dependent elimination v0; reduce.
+    dependent elimination v1; reduce.
+    dependent elimination x0; reduce.
+    dependent elimination x; reduce.
+    now simp Pact_HostExpSem.
+Qed.
+Next Obligation.
+  dependent destruction f.
+  (* FAdd *)
+  - dependent elimination H; reduce.
+    dependent elimination v0; reduce.
+    dependent elimination v1; reduce.
+    dependent elimination x0; reduce.
+    dependent elimination x; reduce.
+    simpl in H0.
+    unfold solution_right in H0.
+    unfold eq_rect_r in H0.
+    unfold eq_rect in H0.
+    simpl in H0.
+    now inversion H0.
+Qed.
+Next Obligation.
+  dependent destruction f.
+  (* FAdd *)
+  - pose proof (ST_AppHost Γ' _ _ FAdd (RenExp σ v) (RenExp_ValueP σ H)).
+    dependent elimination H; reduce.
+    dependent elimination v0; reduce.
+    dependent elimination v1; reduce.
+    dependent elimination x0; reduce.
+    dependent elimination x; reduce.
+    simpl in *.
+    unfold solution_right in H0.
+    unfold eq_rect_r in H0.
+    unfold eq_rect in H0.
+    simpl in H0.
+    now apply H0.
+Qed.
+Next Obligation.
+  dependent destruction f.
+  (* FAdd *)
+  - pose proof (ST_AppHost Γ' _ _ FAdd (SubExp σ v) (SubExp_ValueP σ H)).
+    dependent elimination H; reduce.
+    dependent elimination v0; reduce.
+    dependent elimination v1; reduce.
+    dependent elimination x0; reduce.
+    dependent elimination x; reduce.
+    simpl in *.
+    unfold solution_right in H0.
+    unfold eq_rect_r in H0.
+    unfold eq_rect in H0.
+    simpl in H0.
+    now apply H0.
+Qed.
+Next Obligation.
+  dependent destruction h.
+  (* PInteger *)
+  - now simpl.
+  - now simpl.
+Qed.
+Next Obligation.
+  dependent destruction h.
+  (* PInteger *)
+  - now simpl.
+  - now simpl.
+Qed.
+Next Obligation.
+  dependent destruction h.
+  (* PInteger *)
+  - now constructor.
+  - now constructor.
+Qed.
+Next Obligation.
+  dependent destruction h.
+  (* PInteger *)
+  - now constructor.
+  - now constructor.
+Qed.
+
+Definition num {Γ} (z : Z) : Exp Γ ℤ := HostedVal (PInteger z).
+Arguments num {Γ} z /.
+
 Example exp_constant :
-  run 10 (Constant (LInteger 123%Z)) = MkV (VConst (LInteger 123%Z)).
+  run 10 (num 123) =
+    MkΣ (num 123) Empty MT.
+Proof. reflexivity. Qed.
+
+Example exp_if_true :
+  run 20 (If ETrue (num 123) (num 456)) =
+    MkΣ (num 123) Empty MT.
+Proof. reflexivity. Qed.
+
+Example exp_if_false :
+  run 20 (If EFalse (num 123) (num 456)) =
+    MkΣ (num 456) Empty MT.
 Proof. reflexivity. Qed.
 
 Example exp_pair :
-  run 20 (Pair (Constant (LInteger 123%Z))
-               (Constant (LInteger 456%Z))) =
-    MkV (VPair (VConst (LInteger 123%Z))
-               (VConst (LInteger 456%Z))).
+  run 20 (Pair (num 123) (num 456)) =
+    MkΣ (Pair (num 123) (num 456)) Empty MT.
+Proof. reflexivity. Qed.
+
+Example exp_fst:
+  run 20 (Fst (Pair (num 123) (num 456))) =
+    MkΣ (num 123) Empty MT.
+Proof. reflexivity. Qed.
+
+Example exp_snd :
+  run 20 (Snd (Pair (num 123) (num 456))) =
+    MkΣ (num 456) Empty MT.
+Proof. reflexivity. Qed.
+
+Example exp_list :
+  run 20 (Cons (num 123) (Cons (num 456) Nil)) =
+    MkΣ (Cons (num 123) (Cons (num 456) Nil)) Empty MT.
+Proof. reflexivity. Qed.
+
+Example exp_car:
+  run 20 (Car (num 0) (Cons (num 123) (Cons (num 456) Nil))) =
+    MkΣ (num 123) Empty MT.
+Proof. reflexivity. Qed.
+
+Example exp_car_nil:
+  run 20 (Car (num 0) Nil) =
+    MkΣ (num 0) Empty MT.
+Proof. reflexivity. Qed.
+
+Example exp_cdr :
+  run 20 (Cdr (Cons (num 123) (Cons (num 456) Nil))) =
+    MkΣ (Cons (num 456) Nil) Empty MT.
+Proof. reflexivity. Qed.
+
+Example exp_cdr_nil :
+  run 20 (Cdr (τ:=TyHost TyInteger) Nil) =
+    MkΣ Nil Empty MT.
+Proof. reflexivity. Qed.
+
+Example exp_isnil_cons :
+  run 20 (IsNil (Cons (num 123) (Cons (num 456) Nil))) =
+    MkΣ EFalse Empty MT.
+Proof. reflexivity. Qed.
+
+Example exp_isnil_nil :
+  run 20 (IsNil (τ:=TyHost TyInteger) Nil) =
+    MkΣ ETrue Empty MT.
 Proof. reflexivity. Qed.
 
 Example exp_lam τ :
   run 10 (LAM (cod:=τ) (VAR ZV)) =
-    MkV (VClosure (Lambda (VAR ZV) Empty)).
+    MkΣ (LAM (VAR ZV)) Empty MT.
 Proof. reflexivity. Qed.
 
 Example exp_app :
-  run 10 (APP (LAM (VAR ZV)) (Constant (LInteger 123%Z))) =
-    MkV (VConst (LInteger 123%Z)).
+  run 10 (APP (LAM (VAR ZV)) (num 123)) =
+    MkΣ (num 123) Empty MT.
 Proof. reflexivity. Qed.
+
+Example exp_call_FAdd :
+  run 10 (APP (HostedFun FAdd) (Pair (num 123) (num 456))) =
+    MkΣ (num 579) Empty MT.
+Proof. reflexivity. Qed.
+*)
+
+Compute run 20 (APP (APP (LAM (APP (VAR ZV)
+                             (LAM EUnit)))
+                   (LAM (VAR ZV)))
+              EUnit).
+
+Definition example :
+  run 20 (APP (APP (LAM (APP (VAR ZV)
+                             (LAM EUnit)))
+                   (LAM (VAR ZV)))
+              EUnit).
 
 End Example.
