old/RWSP.v
@@ -11,7 +11,7 @@ Require Import Ltac.
 Generalizable All Variables.
 Set Primitive Projections.
 Set Universe Polymorphism.
-Unset Transparent Obligations.
+(* Unset Transparent Obligations. *)
 
 (******************************************************************************
  * The RWSET Monad transformer
