src/Data/Eq.v
@@ -1,7 +1,7 @@
 Generalizable All Variables.
 Set Primitive Projections.
-Set Universe Polymorphism.
-Unset Transparent Obligations.
+(* Set Universe Polymorphism. *)
+(* Unset Transparent Obligations. *)
 
 Class Eq (A : Type) := {
   eqb  : A -> A -> bool;
