src/Data/Semigroup.v
@@ -2,8 +2,8 @@ Require Import Hask.Prelude.
 
 Generalizable All Variables.
 Set Primitive Projections.
-Set Universe Polymorphism.
-Unset Transparent Obligations.
+(* Set Universe Polymorphism. *)
+(* Unset Transparent Obligations. *)
 
 Class Semigroup (m : Type) := {
   mappend : m -> m -> m;
